src/crypto/aes/ctr.s.dfy
@@ -9,73 +9,28 @@ module CTRModule {
 import opened types_s
 import opened AESModule
 
-function CTR_Encrypt(key:seq<uint32>, input:seq<Quadword>, alg:Algorithm, IV:Quadword) : seq<Quadword>
-    requires |key| == Nk(alg);
-    requires |input| > 0;
-    requires (Nb() * (Nr(alg) + 1)) / 4 == Nr(alg) + 1;   // Easy to prove, but necessary precondition to Cipher
-    requires (Nb() * (Nr(alg) + 1)) % 4 == 0;   // Easy to prove, but necessary precondition to Cipher
-{
-    if |input| == 1 then
-        [AES_Encrypt(key, QuadwordXor(input[0], IV), alg)]
-    else
-        var rest := CTR_Encrypt(key, all_but_last(input), alg, IV);
-        rest + [AES_Encrypt(key, QuadwordXor(last(input), last(rest)), alg)]
-}
+//function CTR_Encrypt_One_Block(key:seq<uint32>, input:Quadword, alg:Algorithm, counter:Quadword) : Quadword
+//    requires |key| == Nk(alg);
+//    requires (Nb() * (Nr(alg) + 1)) / 4 == Nr(alg) + 1;   // Easy to prove, but necessary precondition to Cipher
+//    requires (Nb() * (Nr(alg) + 1)) % 4 == 0;   // Easy to prove, but necessary precondition to Cipher
+//{
+//      QuadwordXor(input, AES_Encrypt(key, counter, alg))
+//}
+//
+//function CTR_EncryptTODO(key:seq<uint32>, input:seq<Quadword>, alg:Algorithm, counter:Quadword) : seq<Quadword>
+//    requires |key| == Nk(alg);
+//    requires |input| > 0;
+//    requires |input| < 0x1_0000_0000_0000_0000;
+//    requires (Nb() * (Nr(alg) + 1)) / 4 == Nr(alg) + 1;   // Easy to prove, but necessary precondition to Cipher
+//    requires (Nb() * (Nr(alg) + 1)) % 4 == 0;   // Easy to prove, but necessary precondition to Cipher
+//{
+//    if |input| == 1 then
+//      [QuadwordXor(input[0], AES_Encrypt(key, counter, alg))]
+//    else
+//      var first := [QuadwordXor(input[0], AES_Encrypt(key, counter, alg))];
+//      var next_counter := CTR_increment_counter(counter);
+//      first + CTR_Encrypt(key, all_but_first(input), alg, next_counter)
+//}
 
-
-function CTR_Decrypt(key:seq<uint32>, input:seq<Quadword>, alg:Algorithm, IV:Quadword) : seq<Quadword>
-    requires |key| == Nk(alg);
-    requires |input| > 0;
-    requires (Nb() * (Nr(alg) + 1)) / 4 == Nr(alg) + 1;   // Easy to prove, but necessary precondition to InvCipher
-    requires (Nb() * (Nr(alg) + 1)) % 4 == 0;   // Easy to prove, but necessary precondition to InvCipher
-{
-    if |input| == 1 then
-        [QuadwordXor(AES_Decrypt(key, input[0], alg), IV)]
-    else
-        var rest := CTR_Decrypt(key, all_but_last(input), alg, IV);
-        rest + [QuadwordXor(AES_Decrypt(key, last(input), alg), input[|input|-2])]
-}
-
-function Uint32ToUint64(low: uint32, high: uint32) : uint64
-{
-  (high * 0x1_0000_0000 + low) as uint64
-}
-
-function Uint64ToUint32(n : uint64) : seq<uint32>
-{
-  [(n / 0x1_0000_0000) as uint32,
-  (n % 0x1_0000_0000) as uint32]
-}
-
-function CTR_increment_counter(counter: Quadword) : Quadword
-{
-  var ctr := Uint32ToUint64(counter.mid_hi,counter.hi); // TODO 
-  var split := Uint64ToUint32(ctr);
-  Quadword(counter.lo,counter.mid_lo, split[0], split[1])
-}
-
-function CTR_Encrypt_One_Block(key:seq<uint32>, input:Quadword, alg:Algorithm, counter:Quadword) : Quadword
-    requires |key| == Nk(alg);
-    requires (Nb() * (Nr(alg) + 1)) / 4 == Nr(alg) + 1;   // Easy to prove, but necessary precondition to Cipher
-    requires (Nb() * (Nr(alg) + 1)) % 4 == 0;   // Easy to prove, but necessary precondition to Cipher
-{
-      QuadwordXor(input, AES_Encrypt(key, counter, alg))
-}
-
-function CTR_EncryptTODO(key:seq<uint32>, input:seq<Quadword>, alg:Algorithm, counter:Quadword) : seq<Quadword>
-    requires |key| == Nk(alg);
-    requires |input| > 0;
-    requires |input| < 0x1_0000_0000_0000_0000;
-    requires (Nb() * (Nr(alg) + 1)) / 4 == Nr(alg) + 1;   // Easy to prove, but necessary precondition to Cipher
-    requires (Nb() * (Nr(alg) + 1)) % 4 == 0;   // Easy to prove, but necessary precondition to Cipher
-{
-    if |input| == 1 then
-      [QuadwordXor(input[0], AES_Encrypt(key, counter, alg))]
-    else
-      var first := [QuadwordXor(input[0], AES_Encrypt(key, counter, alg))];
-      var next_counter := CTR_increment_counter(counter);
-      first + CTR_Encrypt(key, all_but_first(input), alg, next_counter)
-}
-
-// We don't need a decrypt predicate as we are using encrypt again.
+// We don't need a decrypt predicate as the standard uses encrypt again and the xor decrypts.
 }
